# Resources you may find useful

1. [Do your math](https://doyourmath.com)  
2. [Quick math](https://quickmath.com)
3. [Symbolab](https://pt.symbolab.com/solver)
4. [Cymath](https://www.cymath.com/)

## Differential calculus booklet

This huge file will cover solutions for the exercises suggested on [differential calculus booklet](https://drive.google.com/file/d/0B977UW2k4o7acmZ6SkFXZm1LTUk/view). Use the answers as a strategy to understand the necessary steps to solve the problems, not just copy them in a freak way.

### Question No. 1

Use inequalities to describe the given range:

a)
```
-----[-----------)-----
    -2           3
```

b)
```
-----(----------------------->
    -4                       +∞
```

#### Solution for question No. 1

a)
```
  -2 ≤ x < 3
```

b)
```
  x > -4
```

### Question No. 2

Represent the interval given as a line segment on a graduated line:

a) -3 ≤ x < 2  
b) -1 < x < 5  
c) x ≥ 1  
d) 2 ≥ x < 7  

#### Solution for question No. 2

a)
```
----[--------------)-------
   -3              2
```

b)
```
----(--------------------)----
   -1                    5
```

c)
```
-----------[--------------->
           1               +∞
```

d)
```
--------[----------------)----
        2                7
```

### Question No. 3

Determine the distance between two real numbers:

a) 0 and 3  
b) -5 and -2  

#### Solution for question No. 3

a)
```
  3 - 0
  = 3 total distance.
```

b)
```
  (-2) - (-5)
  = 3 total distance
```

### Question No. 4

Determine the interval (s) constituted by the real numbers `x` that satisfy the given inequality:

a) |x - 3| ≤ 1  
b) |2x + 1| > 3  

#### Solution for question No. 4

a)
Developing solution:
```
= |x - 3| ≤ 1
= (x - 3) + 3 ≤ 1 + 3
= x - 3 + 3 ≤ 4
= x ≤ 4
or
= (x - 3) + 3 ≥ -1 + 3
= x - 3 + 3 ≥ 2
= x ≥ 2
```

Presenting solution:
```
S = {x ∈ ℝ | 2 ≤ x ≤ 4}
or
x ∈ [2, 4]
```

b)
Developing solution:
```
= |2x + 1| > 3
= (2x + 1) + (-1) < -3 + (-1)
= 2x + 1 - 1 < -3 - 1
= 2x < -4
= x < -2
or
= (2x + 1) + (-1) > 3 + (-1)
= 2x + 1 - 1 > 3 - 1
= 2x > 2
= x > 1
```

Presenting solution:
```
S = {x ∈ ℝ | x < -2 or x > 1}
or
x ∈ (-∞, -2) ⋃ (1, ∞)
```

### Question No. 5

In the problems presented below, calculate the value of the given expression without using a calculator:

a) 3⁵  
b) 4⁻²  
c) 8 ^ ²⁄₃  
d) 49 ^ ⁻³⁄₂  
e) (4 * (32) ^ ³⁄₄) ÷ (√2)³  
f) (1 ÷ 9) ^ ⁻⁵⁄₂  
g) 16 ^ ³⁄₂ + 27 ^ ²⁄₃  
h) (2 ^ ³⁄₂ * (4 ^ ⁵⁄₂)) ÷ 8 ^ ²⁄₃  
i) (54 ^ (1/3) * 2 ^ (1/6)) ÷ √8  
j) (81 ^ (1/3) * (6 ^ ²⁄₃)) ÷ 2 ^ ⁴⁄₃  


#### Solution for question No. 5

a)
Developing solution:
```
3⁵ = 3 * 3 * 3 * 3 * 3
3⁵ = 27 * 3 * 3
3⁵ = 243
```

b)
Developing solution:
```
4⁻² = (2²) ^ -2
4⁻² = 2 ^ (-2 * 2)
4⁻² = 2 ^ -4
4⁻² = 1 / (2 ^ 4)
4⁻² = 1/16
4⁻² = 0.0625
```

c)
Developing solution:
```
8 ^ ²⁄₃ = (2³) ^ (2/3)
8 ^ ²⁄₃ = 2 ^ (3 * 2/3)
8 ^ ²⁄₃ = 2 ^ ((3 * 2) / 3)
8 ^ ²⁄₃ = 2 ^ (6 / 3)
8 ^ ²⁄₃ = 2 ^ 2
8 ^ ²⁄₃ = 4
```

d)
Developing solution:
```
49 ^ ⁻³⁄₂ = (7²) ^ (-3/2)
49 ^ ⁻³⁄₂ = 7 ^ (2 * -3/2)
49 ^ ⁻³⁄₂ = 7 ^ ((2 * -3) / 2)
49 ^ ⁻³⁄₂ = 7 ^ (-6 / 2)
49 ^ ⁻³⁄₂ = 7 ^ (-3)
49 ^ ⁻³⁄₂ = 1 / (7 ^ 3)
49 ^ ⁻³⁄₂ = 1 / 343
49 ^ ⁻³⁄₂ ≈ 0.0029
```

e)
Developing solution:
```
(4 * (32) ^ ³⁄₄) ÷ (√2)³ = (4 * (2⁵) ^ (3/4)) ÷ (√2) ^ 3
(4 * (32) ^ ³⁄₄) ÷ (√2)³ = (4 * 2 ^ (5 * 3/4)) ÷ (√2) ^ 3
(4 * (32) ^ ³⁄₄) ÷ (√2)³ = (4 * 2 ^ ((5 * 3) / 4)) ÷ (√2) ^ 3
(4 * (32) ^ ³⁄₄) ÷ (√2)³ = (4 * 2 ^ (15/4)) ÷ (√2) ^ 3
(4 * (32) ^ ³⁄₄) ÷ (√2)³ = (4 * 2 ^ (15/4)) ÷ (2 ^ (1/2)) ^ 3
(4 * (32) ^ ³⁄₄) ÷ (√2)³ = (4 * 2 ^ (15/4)) ÷ 2 ^ ((1/2) * 3)
(4 * (32) ^ ³⁄₄) ÷ (√2)³ = (4 * 2 ^ (15/4)) ÷ 2 ^ ((1 * 3) / 2)
(4 * (32) ^ ³⁄₄) ÷ (√2)³ = (4 * 2 ^ (15/4)) ÷ 2 ^ (3/2)
(4 * (32) ^ ³⁄₄) ÷ (√2)³ = (4 * 2 ^ (15/4)) ÷ (2 * 2 ^ (1/2))
(4 * (32) ^ ³⁄₄) ÷ (√2)³ = ((2²) * 2 ^ (15/4)) ÷ (2 * 2 ^ (1/2))
(4 * (32) ^ ³⁄₄) ÷ (√2)³ = (2 * 2 ^ (15/4)) ÷ (2 ^ (1/2))
(4 * (32) ^ ³⁄₄) ÷ (√2)³ = 2 * 2 ^ ((15/4) - (1/2))
(4 * (32) ^ ³⁄₄) ÷ (√2)³ = 2 * 2 ^ ((15/4) - (2/4))
(4 * (32) ^ ³⁄₄) ÷ (√2)³ = 2 * 2 ^ (13/4)
(4 * (32) ^ ³⁄₄) ÷ (√2)³ = 2 * 2 ^ 3 * 2 ^ (1/4)
(4 * (32) ^ ³⁄₄) ÷ (√2)³ = 2 ^ 4 * 2 ^ (1/4)
(4 * (32) ^ ³⁄₄) ÷ (√2)³ = 16 * 2 ^ (1/4)
(4 * (32) ^ ³⁄₄) ÷ (√2)³ ≈ 19.0273
```

f)
Developing solution:
```
(1 ÷ 9) ^ ⁻⁵⁄₂ = 1 ÷ ((1/9) ^ (5/2))
(1 ÷ 9) ^ ⁻⁵⁄₂ = 1 ÷ (1 ^ (5/2) / 9 ^ (5/2))
(1 ÷ 9) ^ ⁻⁵⁄₂ = 1 ÷ (1 / 9 ^ (5/2))
(1 ÷ 9) ^ ⁻⁵⁄₂ = 1 ÷ (1 / (3²) ^ (5/2))
(1 ÷ 9) ^ ⁻⁵⁄₂ = 1 ÷ (1 / 3 ^ (2 * (5/2)))
(1 ÷ 9) ^ ⁻⁵⁄₂ = 1 ÷ (1 / 3 ^ ((2 * 5) / 2))
(1 ÷ 9) ^ ⁻⁵⁄₂ = 1 ÷ (1 / 3 ^ (10/2))
(1 ÷ 9) ^ ⁻⁵⁄₂ = 1 ÷ (1 / 3 ^ 5)
(1 ÷ 9) ^ ⁻⁵⁄₂ = 1 ÷ (1/243)
(1 ÷ 9) ^ ⁻⁵⁄₂ = 243 ÷ 1
(1 ÷ 9) ^ ⁻⁵⁄₂ = 243
```

g)
Developing solution:
```
16 ^ ³⁄₂ + 27 ^ ²⁄₃ = (2⁴) ^ (3/2) + (3³) ^ (2/3)
16 ^ ³⁄₂ + 27 ^ ²⁄₃ = 2 ^ (4 * (3/2)) + 3 ^ (3 * (2/3))
16 ^ ³⁄₂ + 27 ^ ²⁄₃ = 2 ^ ((4 * 3) / 2) + 3 ^ ((3 * 2) / 3)
16 ^ ³⁄₂ + 27 ^ ²⁄₃ = 2 ^ (12/2) + 3 ^ (6/3)
16 ^ ³⁄₂ + 27 ^ ²⁄₃ = 2 ^ 6 + 3 ^ 2
16 ^ ³⁄₂ + 27 ^ ²⁄₃ = 64 + 9
16 ^ ³⁄₂ + 27 ^ ²⁄₃ = 73
```

h)
Developing solution:
```
(2 ^ ³⁄₂ * (4 ^ ⁵⁄₂)) ÷ 8 ^ ²⁄₃ = (2 ^ (3/2) * ((2²) ^ (5/2))) ÷ 8 ^ (2/3)
(2 ^ ³⁄₂ * (4 ^ ⁵⁄₂)) ÷ 8 ^ ²⁄₃ = (2 ^ (3/2) * (2 ^ (2 * (5/2)))) ÷ 8 ^ (2/3)
(2 ^ ³⁄₂ * (4 ^ ⁵⁄₂)) ÷ 8 ^ ²⁄₃ = (2 ^ (3/2) * (2 ^ ((2 * 5) / 2))) ÷ 8 ^ (2/3)
(2 ^ ³⁄₂ * (4 ^ ⁵⁄₂)) ÷ 8 ^ ²⁄₃ = (2 ^ (3/2) * (2 ^ (10/2))) ÷ 8 ^ (2/3)
(2 ^ ³⁄₂ * (4 ^ ⁵⁄₂)) ÷ 8 ^ ²⁄₃ = (2 ^ (3/2) * (2 ^ 5)) ÷ 8 ^ (2/3)
(2 ^ ³⁄₂ * (4 ^ ⁵⁄₂)) ÷ 8 ^ ²⁄₃ = (2 ^ (3/2) * 2 ^ 5) ÷ ((2³) ^ (2/3))
(2 ^ ³⁄₂ * (4 ^ ⁵⁄₂)) ÷ 8 ^ ²⁄₃ = (2 ^ (3/2) * 2 ^ 5) ÷ (2 ^ (3 * (2/3)))
(2 ^ ³⁄₂ * (4 ^ ⁵⁄₂)) ÷ 8 ^ ²⁄₃ = (2 ^ (3/2) * 2 ^ 5) ÷ (2 ^ ((3 * 2) / 3))
(2 ^ ³⁄₂ * (4 ^ ⁵⁄₂)) ÷ 8 ^ ²⁄₃ = (2 ^ (3/2) * 2 ^ 5) ÷ (2 ^ (6/3))
(2 ^ ³⁄₂ * (4 ^ ⁵⁄₂)) ÷ 8 ^ ²⁄₃ = (2 ^ (3/2) * 2 ^ 5) ÷ (2 ^ 2)
(2 ^ ³⁄₂ * (4 ^ ⁵⁄₂)) ÷ 8 ^ ²⁄₃ = 2 ^ 5 ÷ (2 ^ (2 - (3/2)))
(2 ^ ³⁄₂ * (4 ^ ⁵⁄₂)) ÷ 8 ^ ²⁄₃ = 2 ^ 5 ÷ 2 ^ (1/2)
(2 ^ ³⁄₂ * (4 ^ ⁵⁄₂)) ÷ 8 ^ ²⁄₃ = 2 ^ (5 - (1/2))
(2 ^ ³⁄₂ * (4 ^ ⁵⁄₂)) ÷ 8 ^ ²⁄₃ = 2 ^ (9/2)
(2 ^ ³⁄₂ * (4 ^ ⁵⁄₂)) ÷ 8 ^ ²⁄₃ = 2 ^ (4 + (1/2))
(2 ^ ³⁄₂ * (4 ^ ⁵⁄₂)) ÷ 8 ^ ²⁄₃ = 2 ^ 4 * 2 ^ (1/2)
(2 ^ ³⁄₂ * (4 ^ ⁵⁄₂)) ÷ 8 ^ ²⁄₃ = 16 * 2 ^ (1/2)
(2 ^ ³⁄₂ * (4 ^ ⁵⁄₂)) ÷ 8 ^ ²⁄₃ ≈ 22.6274
```

i)
Developing solution:
```
(³√54 * ⁶√2) ÷ √8 = (³√54 * ⁶√2) ÷ √2³
(³√54 * ⁶√2) ÷ √8 = (³√54 * ⁶√2) ÷ √2²*2¹
(³√54 * ⁶√2) ÷ √8 = (³√54 * ⁶√2) ÷ √2² * √2¹
(³√54 * ⁶√2) ÷ √8 = (³√54 * ⁶√2) ÷ 2 * √2¹
(³√54 * ⁶√2) ÷ √8 = (³√54 * ⁶√2) ÷ 2 * √2
(³√54 * ⁶√2) ÷ √8 = (³√3³*2 * ⁶√2) ÷ 2 * √2
(³√54 * ⁶√2) ÷ √8 = (³√3³ * ³√2 * ⁶√2) ÷ 2 * √2
(³√54 * ⁶√2) ÷ √8 = (3 * ³√2 * ⁶√2) ÷ 2 * √2
(³√54 * ⁶√2) ÷ √8 = 3 * 2 ^ ((1/3) + (1/6)) ÷ 2 * √2
(³√54 * ⁶√2) ÷ √8 = 3 * 2 ^ (9/18) ÷ 2 * √2
(³√54 * ⁶√2) ÷ √8 = 3 * 2 ^ (1/2) ÷ 2 * √2
(³√54 * ⁶√2) ÷ √8 = 3 * √2 ÷ 2 * √2
(³√54 * ⁶√2) ÷ √8 = 3 ÷ 2
(³√54 * ⁶√2) ÷ √8 = 1.5
```

j)
Developing solution:
```
(³√81 * (6 ^ ²⁄₃)) ÷ 2 ^ ⁴⁄₃ = (³√81 * (6 ^ (2/3))) ÷ 2 ^ (4/3)
(³√81 * (6 ^ ²⁄₃)) ÷ 2 ^ ⁴⁄₃ = (³√81 * (2 ^ (2/3) * 3 ^ (2/3))) ÷ 2 ^ (4/3)
(³√81 * (6 ^ ²⁄₃)) ÷ 2 ^ ⁴⁄₃ = (81 ^ (1/3) * 2 ^ (2/3) * 3 ^ (2/3)) ÷ 2 ^ (4/3)
(³√81 * (6 ^ ²⁄₃)) ÷ 2 ^ ⁴⁄₃ = (81 ^ (1/3) * 3 ^ (2/3)) ÷ 2 ^ ((4/3) - (2/3))
(³√81 * (6 ^ ²⁄₃)) ÷ 2 ^ ⁴⁄₃ = (81 ^ (1/3) * 3 ^ (2/3)) ÷ 2 ^ (2/3)
(³√81 * (6 ^ ²⁄₃)) ÷ 2 ^ ⁴⁄₃ = ((3⁴) ^ (1/3) * 3 ^ (2/3)) ÷ 2 ^ (2/3)
(³√81 * (6 ^ ²⁄₃)) ÷ 2 ^ ⁴⁄₃ = (3 ^ (4 * (1/3)) * 3 ^ (2/3)) ÷ 2 ^ (2/3)
(³√81 * (6 ^ ²⁄₃)) ÷ 2 ^ ⁴⁄₃ = (3 ^ ((4 * 1) / 3) * 3 ^ (2/3)) ÷ 2 ^ (2/3)
(³√81 * (6 ^ ²⁄₃)) ÷ 2 ^ ⁴⁄₃ = (3 ^ (4/3) * 3 ^ (2/3)) ÷ 2 ^ (2/3)
(³√81 * (6 ^ ²⁄₃)) ÷ 2 ^ ⁴⁄₃ = (3 ^ ((4/3) + (2/3))) ÷ 2 ^ (2/3)
(³√81 * (6 ^ ²⁄₃)) ÷ 2 ^ ⁴⁄₃ = 3 ^ (6/3) ÷ 2 ^ (2/3)
(³√81 * (6 ^ ²⁄₃)) ÷ 2 ^ ⁴⁄₃ = 3 ^ 2 ÷ 2 ^ (2/3)
(³√81 * (6 ^ ²⁄₃)) ÷ 2 ^ ⁴⁄₃ = 9 ÷ 2 ^ (2/3)
(³√81 * (6 ^ ²⁄₃)) ÷ 2 ^ ⁴⁄₃ ≈ 5.6696
```
