# Validating essential math exercises

Remote exam.

## Summary

- [Question No. 1](https://github.com/Bodera/learnPath_Mathematics/blob/master/statistics/1st-validation.md#question-no-1)
- [Question No. 2](https://github.com/Bodera/learnPath_Mathematics/blob/master/statistics/1st-validation.md#question-no-2)
- [Question No. 3](https://github.com/Bodera/learnPath_Mathematics/blob/master/statistics/1st-validation.md#question-no-3)
- [Question No. 4](https://github.com/Bodera/learnPath_Mathematics/blob/master/statistics/1st-validation.md#question-no-4)
- [Question No. 5](https://github.com/Bodera/learnPath_Mathematics/blob/master/statistics/1st-validation.md#question-no-5)
- [Question No. 6](https://github.com/Bodera/learnPath_Mathematics/blob/master/statistics/1st-validation.md#question-no-6)
- [Question No. 7](https://github.com/Bodera/learnPath_Mathematics/blob/master/statistics/1st-validation.md#question-no-7)
- [Question No. 8](https://github.com/Bodera/learnPath_Mathematics/blob/master/statistics/1st-validation.md#question-no-8)
- [Question No. 9](https://github.com/Bodera/learnPath_Mathematics/blob/master/statistics/1st-validation.md#question-no-9)
- [Question No. 10](https://github.com/Bodera/learnPath_Mathematics/blob/master/statistics/1st-validation.md#question-no-10)

### Question No. 1

The value of the expression below is?

```txt
(4⁷ * 4¹⁰ * 4)² ÷ (4⁵)⁷
```

#### Procedures for solution of question No. 1

__1st step__: Simplify amap (*as much as possible*).

```txt
(4⁷ * 4¹⁰ * 4)² ÷ (4⁵)⁷
= (4⁷⁺¹⁰⁺¹)² ÷ (4⁵)⁷
= (4¹⁸)² ÷ (4⁵)⁷
= 4¹⁸*² ÷ 4⁵*⁷
= 4³⁶ ÷ 4³⁵
= 4³⁶⁻³⁵
= 4¹
= 4
```

__2nd step__: Answer the question.

The answer is `4`.

### Question No. 2

Calculate:

![Question No. 2 problem](https://latex.codecogs.com/svg.latex?\left&space;[&space;\left&space;(&space;\frac{1}{3}&space;-&space;\frac{1}{4}&space;\right&space;)&space;\div&space;\frac{7}{12}&space;&plus;&space;\frac{1}{7}&space;\times&space;\left&space;(&space;\frac{7}{2}&space;-&space;\frac{5}{2}&space;\right&space;)&space;\right&space;]&space;\times&space;\frac{1}{2}&space;\div&space;\frac{1}{7})

#### Procedures for solution of question No. 2

__1st step__: Solve the parentheses first.

```txt
[(¹⁄₃ - ¹⁄₄) ÷ ⁷⁄₁₂ + ¹⁄₇ * (⁷⁄₂ - ⁵⁄₂)] * ¹⁄₂ ÷ ¹⁄₇
= [(¹⁄₃ - ¹⁄₄) ÷ ⁷⁄₁₂ + ¹⁄₇ * (²⁄₂)] * ¹⁄₂ ÷ ¹⁄₇
= [(⁴⁄₁₂ - ³⁄₁₂) * 12 ÷ 7 + ¹⁄₇ * 1] * ¹⁄₂ ÷ ¹⁄₇ //fractions property a ÷ b ÷ c = a * c ÷ b
= [¹⁄₁₂ * 12 ÷ 7 + ¹⁄₇ * 1] * ¹⁄₂ ÷ ¹⁄₇
= [¹²⁄₁₂ ÷ 7 + ¹⁄₇ * 1] * ¹⁄₂ ÷ ¹⁄₇
= [1 ÷ 7 + ¹⁄₇ * 1] * ¹⁄₂ ÷ ¹⁄₇
= [¹⁄₇ + ¹⁄₇ * 1] * ¹⁄₂ ÷ ¹⁄₇
= ²⁄₇ * ⁷⁄₂ //fractions property a ÷ b ÷ c ÷ d = a * d ÷ b * c
= ¹⁴⁄₁₄
= 1
```

__2nd step__: Answer the question.

The answer is `1`.

### Question No. 3

What is the result of simplifying the expression below?

![Question No. 3 problem](https://latex.codecogs.com/svg.latex?\left&space;(&space;\frac{x^{3}&space;\times&space;x^{10}&space;\times&space;x^{5}}{x^{5}&space;\times&space;x^{2}}&space;\right&space;)^{2})

#### Procedures for solution of question No. 3

__1st step__: Simplify by applying the exponents properties.

```txt
((x³ * x¹⁰ * x⁵) ÷ (x⁵ * x²))²
= (((x³)² * (x¹⁰)² * (x⁵)²) ÷ ((x⁵)² * (x²)²))
= ((x⁶ * x²⁰ * x¹⁰) ÷ (x¹⁰ * x⁴))
= x³⁶ ÷ x¹⁴
= x²²
```

__2nd step__: Answer the question.

The answer is `x²²`.

### Question No. 4

Given the values of __a__ and __b__ below, the result of the quotient __a/b__ is?

```txt
a = 2⁷ * 3⁸ * 7
b = 2⁵ * 3⁶
```

#### Procedures for solution of question No. 4

__1st step__: Calculate the values of __a__ and __b__.

```txt
a = 128 * 6561 * 7
b = 32 * 729

a = 5878656
b = 23328
```

__2nd step__: Calculate the quotient.

```txt
a/b = 5878656 ÷ 23328
a/b = 252
```

__3rd step__: Answer the question.

The answer is `252`.

### Question No. 5

Solve the 2nd degree equation below and report the solution in the set of real numbers.

```txt
3x² - 2x - 1 = 0
```

#### Procedures for solution of question No. 5

__1st step__: Remember quadratic formula.

```txt
x = (-b ± √Δ) ÷ 2a
Δ = b² - 4ac
```

__2nd step__: Calculate the equation.

```txt
Δ = (-2)² - (4 * 3 * (-1))
Δ = 4 - (-12)
Δ = 16

x = (-(-2) ± √16) ÷ (2 * 3)
x = (2 ± 4) ÷ 6

x' = (2 + 4) ÷ 6
x' = 6 ÷ 6
x' = 1

x'' = (2 - 4) ÷ 6
x'' = -2 ÷ 6
x'' = -⅓
```

__3rd step__: Answer the question.

The solution ∈ ℝ is `S={1; -⅓}`.

### Question No. 6

Calculate:

![Question No. 6 problem](https://latex.codecogs.com/svg.latex?\frac{\frac{1}{3}&plus;\frac{2}{5}&plus;\frac{1}{30}}{\frac{23}{30}})

#### Procedures for solution of question No. 6

__1st step__: Remember the properties of fractions.

```txt
((1÷3) + (2÷5) + (1÷30)) ÷ (23÷30)
= ((5÷15) + (6÷15) + (1÷30)) ÷ (23÷30)
= ((11÷15) + (1÷30)) ÷ (23÷30)
= ((44÷60) + (2÷60)) ÷ (23÷30)
= (46÷60) ÷ (23÷30)
= (46÷60) ÷ (23÷30)
= (46 * 30) ÷ (23 * 60)
= 1380 ÷ 1380
= 1
```

__2nd step__: Answer the question.

The answer is `1`.

### Question No. 7

Calculate:

![Question No. 7 problem](https://latex.codecogs.com/svg.latex?\sqrt{4}&space;&plus;&space;\sqrt{64}&space;&plus;&space;\left(&space;-\sqrt{144}&space;\right)&space;&plus;&space;\sqrt[3]{8}&space;&plus;&space;\sqrt[3]{-8}&space;&plus;&space;\sqrt[3]{125}&space;&plus;&space;\left(-\sqrt[3]{-8}&space;\right)&space;&plus;&space;\sqrt[4]{256}&space;&plus;&space;\sqrt[4]{1296}&space;&plus;&space;\left(&space;-\sqrt[3]{729}&space;\right)&space;&plus;&space;\sqrt{0,01}&space;&plus;&space;\sqrt[3]{-0,001})

#### Procedures for solution of question No. 7

__1st step__: Find the result of the radicals then add it all up.

```txt
√4 + √64 + (-√144) + ³√8 + ³√-8 + ³√125 + (-³√-8) + ⁴√256 + ⁴√1296 + (-³√729) + √0.01 + ³√-0.001
= 2 + 8 + (-12) + 2 + (-2) + 5 + 2 + 4 + 6 + (-9) + 0.1 + (-0.1)
= 29.1 + (-23.1)
= 6
```

__2nd step__: Answer the question.

The answer is `6`.

### Question No. 8

Calculate:

![Question No. 8 problem](https://latex.codecogs.com/svg.latex?\frac{10x&space;-&space;4}{6}&space;=&space;\frac{8x&space;-&space;20}{4})

#### Procedures for solution of question No. 8

__1st step__: Solve the equation using cross-multiplication of fractions.

```txt
(10x - 4) ÷ 6 = (8x - 20) ÷ 4
4 * (10x - 4) = 6 * (8x - 20) //if a/b = c/d then a*d = b*c
40x - 16 = 48x - 120
40x - 48x = (-120) + 16
-8x = -104
-x = (-104) ÷ 8
-x = -13
x = 13
```

__2nd step__: Answer the question.

The answer is `13`.

### Question No. 9

The sum of __x__ and __y__ that represent the solution of the system of equations below is?

![Question No. 9 problem](https://latex.codecogs.com/svg.latex?\left\{\begin{matrix}&space;4x&space;-&space;\left&space;(&space;y&space;\div&space;2&space;\right&space;)&space;=&space;-\left&space;(&space;25&space;\div&space;2&space;\right&space;)&space;\\&space;2(x&plus;1)&space;&plus;&space;5&space;=&space;y&space;\end{matrix}\right.)

#### Procedures for solution of question No. 9

__1st step__: Isolate one variable from the equation.

```txt
4x - (y ÷ 2) = -(25 ÷ 2)
2(x+1) + 5 = y

//let's isolate 4x 1st.
4x - (y ÷ 2) = -(25 ÷ 2)
4x - (y ÷ 2) = -(25 ÷ 2) + (y ÷ 2)
4x = -(25 ÷ 2) + (y ÷ 2)
4x = (-25 + y) ÷ 2
x = ((y - 25) ÷ 2) ÷ 4 //b ÷ c ÷ a = b ÷ c * a
x = (y - 25) ÷ (2 * 4)
x = (y - 25) ÷ 8

//now we're going to discover the value o y.
2(x+1) + 5 = y
2 * (((y - 25) ÷ 8) + 1) + 5 = y
2 * (((y - 25) ÷ 8) + 1) = y - 5
(((y - 25) * 2 ÷ 8 * 1) + 1 * 2) = y - 5
((y - 25) * 2 ÷ 8) + 2 = y - 5
(y - 25) ÷ 4 + 2 = y - 5
(y - 25) ÷ 4 + 2 = y - 5 - y
(y - 25) ÷ 4 + 2 - y = -5
(y - 25) ÷ 4 - y = -5 - 2
(y - 25) ÷ 4 - y = -7
(y - 25) ÷ 4 - (y * 4) ÷ 4 = -7
(y - 25 - y * 4) ÷ 4 = -7
(y - 25 - 4y) ÷ 4 = -7
(-25 - 3y) ÷ 4 = -7
(-25 - 3y) * 4 ÷ 4 = (-7) * 4
-25 - 3y = -28
-3y = -28 + 25
-3y = -3
-3y ÷ -3 = -3 ÷ -3
y = 1

//finally we replace y in x.
x = (y - 25) ÷ 8
x = (1 - 25) ÷ 8
x = - 24 ÷ 8
x = -3

//sum the value of the variables x and y.
-3 + 1
= -2
```

__2nd step__: Answer the question.

The answer is `-2`.

### Question No. 10

Solve the equation below and report the solution in the set of real numbers.

![Question No. 10 problem](https://latex.codecogs.com/svg.latex?2&space;&plus;&space;3[x&space;-&space;(3x&space;&plus;&space;1)]&space;=&space;5[x&space;-&space;(2x-1)])

#### Procedures for solution of question No. 10

__1st step__: Expand the equalities.

```txt
2 + 3[x-(3x + 1)] = 5[x-(2x-1)]
2 + 3[x - 3x - 1] = 5[x - 2x + 1]
2 + 3[-2x - 1] = 5[-x + 1]
2 + -6x - 3 = -5x + 5
-6x - 1 = -5x + 5
-6x + 5x = 1 + 5
-x = 6
x = -6
```

__2nd step__: Answer the question.

The solution ∈ ℝ is `S={-6}`.
