# Fractional numbers and numeric expressions

## Series No. I

Simplify:

I) ğŸ ª â¸â„â‚‚â‚„  
II) ğŸ ª Â²Â¹â„â‚‚â‚ˆ  
III) ğŸ ª Â³Â²â„â‚„â‚€  
IV) ğŸ ª â´â¸â„â‚ˆâ‚„  

### Resolution for series no. I

```txt
gcd(8;24)

Factors of 8 = 2 ^ 3
Factors of 24 = 2 ^ 3 * 3

Thus gcd(8;24) = 2^3 = 8

8 Ã· 8 = 1
24 Ã· 8 = 3

â¸â„â‚‚â‚„ = â…“
```

```txt
gcd(21;28)

Factors of 21 = 3 * 7
Factors of 28 = 2 ^ 2 * 7

Thus gcd(8;24) = 7

21 Ã· 7 = 3
28 Ã· 7 = 4

Â²Â¹â„â‚‚â‚ˆ = Â¾
```

```txt
gcd(32;40)

Factors of 32 = 2 ^ 5
Factors of 40 = 2 ^ 3 * 5

Thus gcd(32;40) = 2 ^ 3 = 8

32 Ã· 8 = 4
40 Ã· 8 = 5

Â³Â²â„â‚„â‚€ = â…˜
```

```txt
gcd(48;84)

Factors of 48 = 2 ^ 4 * 3
Factors of 84 = 2 ^ 2 * 3 * 7

Thus gcd(48;84) = 2 ^ 2 * 3 = 12

48 Ã· 12 = 4
84 Ã· 12 = 7

â´â¸â„â‚ˆâ‚„ = â´â„â‚‡
```

## Series No. II

Write as a mixed fraction:

I) ğŸ ª Â³Â¹â„â‚…  
II) ğŸ ª Â²â´â„â‚‡  
III) ğŸ ª Â²Â³â„â‚…  
IV) ğŸ ª â´Â¹â„â‚‰  

### Resolution for series no. II

```txt
31 Ã· 5 = 6 with remainder of 1

Thus Â³Â¹â„â‚… = 6â…•
```

```txt
24 Ã· 7 = 3 with remainder of 3

Thus Â²â´â„â‚‡ = 3Â³â„â‚‡
```

```txt
23 Ã· 5 = 4 with remainder of 3

Thus Â²Â³â„â‚… = 4â…—
```

```txt
41 Ã· 9 = 4 with remainder of 5

Thus â´Â¹â„â‚‰ = 4âµâ„â‚‰
```

## Series No. III

Write as a fraction:

I) ğŸ ª 3â…š  
II) ğŸ ª 1â´â„â‚‡  
III) ğŸ ª 2â…“  
IV) ğŸ ª 7Â½  

### Resolution for series no. III

```txt
3â…š  = (6 * 3 + 5) Ã· 6
    = 23 Ã· 6

Thus 3â…š = Â²Â³â„â‚†
```

```txt
1â´â„â‚‡ = (7 * 1 + 4) Ã· 7
    = 11 Ã· 7

Thus 1â´â„â‚‡ = Â¹Â¹â„â‚‡
```

```txt
2â…“  = (3 * 2 + 1) Ã· 3
    = 7 Ã· 3

Thus 2â…“ = â·â„â‚ƒ
```

```txt
7Â½  = (2 * 7 + 1) Ã· 2
    = 15 Ã· 2

Thus 7Â½ = Â¹âµâ„â‚‚
```

## Series No. IV

Resolve:

I) ğŸ ª â·â„â‚â‚ƒ + Â¹â°â„â‚â‚ƒ  
II) ğŸ ª â¹â„â‚â‚ + Â¹â°â„â‚â‚  
III) ğŸ ª 2â…• + â…–  
IV) ğŸ ª 1Â³â„â‚â‚€ + 2â¹â„â‚â‚€  

### Resolution for series no. IV

```txt
â·â„â‚â‚ƒ + Â¹â°â„â‚â‚ƒ =  â½â·âºÂ¹â°â¾â„â‚â‚ƒ
            = Â¹â·â„â‚â‚ƒ
            = 1â´â„â‚â‚ƒ

Thus â·â„â‚â‚ƒ + Â¹â°â„â‚â‚ƒ = 1â´â„â‚â‚ƒ
```

```txt
â¹â„â‚â‚ + Â¹â°â„â‚â‚ = â½â¹âºÂ¹â°â¾â„â‚â‚
            = Â¹â¹â„â‚â‚
            = 1â¸â„â‚â‚

Thus â¹â„â‚â‚ + Â¹â°â„â‚â‚ = 1â¸â„â‚â‚
```

```txt
2â…• + â…– = Â¹Â¹â„â‚… + â…–
       = â½Â¹Â¹âºÂ²â¾â„â‚…
       = Â¹Â³â„â‚…
       = 2â…—

Thus 2â…• + â…– = 2â…—
```

```txt
1Â³â„â‚â‚€ + 2â¹â„â‚â‚€ = Â¹Â³â„â‚â‚€ + Â²â¹â„â‚â‚€
             = â½Â¹Â³âºÂ²â¹â¾â„â‚â‚€
             = â´Â²â„â‚â‚€
             = Â²Â¹â„â‚…
             = 4Â¹â„â‚…

Thus 1Â³â„â‚â‚€ + 2â¹â„â‚â‚€ = 4Â¹â„â‚…
```

## Series No. V

Resolve:

I) ğŸ ª â¸â„â‚â‚… - Â²â„â‚â‚…  
II) ğŸ ª Â¹â°â„â‚ƒ - 2â…“  
III) ğŸ ª 5â…™ - 2â…š  
IV) ğŸ ª 2Â³â„â‚‡ - 1â…  

### Resolution for series no. V

```txt
â¸â„â‚â‚… - Â²â„â‚â‚…  = â½â¸â»Â²â¾â„â‚â‚…
            = â¶â„â‚â‚…
            = Â²â„â‚…

Thus â¸â„â‚â‚… - Â²â„â‚â‚… = Â²â„â‚…
```

```txt
Â¹â°â„â‚ƒ - 2â…“  = Â¹â°â„â‚ƒ - â·â„â‚ƒ
           = â½Â¹â°â»â·â¾â„â‚ƒ
           = Â³â„â‚ƒ
           = 1

Thus Â¹â°â„â‚ƒ - 2â…“ = 1
```

```txt
5â…™ - 2â…š    = Â³Â¹â„â‚† - Â¹â·â„â‚†
           = â½Â³Â¹â»Â¹â·â¾â„â‚†
           = Â¹â´â„â‚†
           = â·â„â‚ƒ
           = 2Â¹â„â‚ƒ

Thus 5â…™ - 2â…š = 2Â¹â„â‚ƒ
```

```txt
2Â³â„â‚‡ - 1â…  = Â¹â·â„â‚‡ - â¸â„â‚‡
           = â½Â¹â·â»â¸â¾â„â‚‡
           = â¹â„â‚‡
           = 1Â²â„â‚‡

Thus 2Â³â„â‚‡ - 1â… = 1Â²â„â‚‡
```

## Series No. VI

Resolve:

I) ğŸ ª â¸â„â‚â‚ƒ + Â¹â°â„â‚â‚ƒ - â·â„â‚â‚ƒ  
II) ğŸ ª 1Â³â„â‚… + â´â„â‚… - Â²â„â‚…  
III) ğŸ ª Â¹â¹â„â‚‡ - Â²â„â‚‡ + Â³â„â‚‡  
IV) ğŸ ª 1âµâ„â‚† - Â¹â„â‚† + âµâ„â‚†  

### Resolution for series no. VI

```txt
â¸â„â‚â‚ƒ + Â¹â°â„â‚â‚ƒ - â·â„â‚â‚ƒ   = â½â¸âºÂ¹â°â»â·â¾â„â‚â‚ƒ
                    = Â¹Â¹â„â‚â‚ƒ

Thus â¸â„â‚â‚ƒ + Â¹â°â„â‚â‚ƒ - â·â„â‚â‚ƒ = Â¹Â¹â„â‚â‚ƒ
```

```txt
1Â³â„â‚… + â´â„â‚… - Â²â„â‚…  = â½â¸âºâ´â»Â²â¾â„â‚…
                = Â¹â°â„â‚…
                = 2

Thus 1Â³â„â‚… + â´â„â‚… - Â²â„â‚… = 2
```

```txt
Â¹â¹â„â‚‡ - Â²â„â‚‡ + Â³â„â‚‡  = â½Â¹â¹â»Â²âºÂ³â¾â„â‚‡
                = Â²â°â„â‚‡
                = 2â¶â„â‚‡

Thus Â¹â¹â„â‚‡ - Â²â„â‚‡ + Â³â„â‚‡ = 2â¶â„â‚‡
```

```txt
1âµâ„â‚† - Â¹â„â‚† + âµâ„â‚†  = â½Â¹Â¹â»Â¹âºâµâ¾â„â‚†
                = Â¹âµâ„â‚†
                = âµâ„â‚‚
                = 2Â¹â„â‚‚

Thus 1âµâ„â‚† - Â¹â„â‚† + âµâ„â‚† = 2Â¹â„â‚‚
```

## Series No. VII

Resolve:

I) ğŸ ª Â¹â„â‚ƒ + Â²â„â‚…  
II) ğŸ ª 3Â¹â„â‚‚ + Â²â„â‚ƒ  
III) ğŸ ª 2 + Â¹â„â‚„  
IV) ğŸ ª 1 + Â³â„â‚‡  

### Resolution for series no. VII

```txt
lcd(3;5)

Factors of 3 = 3
Factors of 5 = 5

Thus lcd(3;5) = 3 * 5 = 15 (so denominator must be 15)

multiplying fractions in cross:

Â¹â„â‚ƒ + Â²â„â‚… becomes âµâ„â‚â‚… + â¶â„â‚â‚… (makes total sense)

âµâ„â‚â‚… + â¶â„â‚â‚… = â½âµâºâ¶â¾â„â‚â‚…
           = Â¹Â¹â„â‚â‚…

Thus Â¹â„â‚ƒ + Â²â„â‚… = Â¹Â¹â„â‚â‚…
```

```txt
lcd(2;3)

Factors of 2 = 2
Factors of 3 = 3

Thus lcd(2;3) = 2 * 3 = 6 (so denominator must be 6)

multiplying fractions in cross:

3Â¹â„â‚‚ + Â²â„â‚ƒ = â·â„â‚‚ + Â²â„â‚ƒ

â·â„â‚‚ + Â²â„â‚ƒ becomes Â²Â¹â„â‚† + â´â„â‚† (makes total sense)

Â²Â¹â„â‚â‚‚ + â´â„â‚â‚‚ = â½Â²Â¹âºâ´â¾â„â‚†
            = Â²âµâ„â‚†
            = 4Â¹â„â‚†

Thus 3Â¹â„â‚‚ + Â²â„â‚ƒ = 4Â¹â„â‚†
```

```txt
lcd(1;4)

Factors of 1 = 1
Factors of 4 = 2 ^ 2

Thus lcd(1;4) = 2 ^ 2 * 1 = 4 (so denominator must be 4)

multiplying fractions in cross:

2 + Â¹â„â‚„ becomes â¸â„â‚„ + Â¹â„â‚„ (makes total sense)

â¸â„â‚„ + Â¹â„â‚„ = â½â¸âºÂ¹â¾â„â‚„
         = â¹â„â‚„
         = 2Â¹â„â‚„

Thus 2 + Â¹â„â‚„ = 2Â¹â„â‚„
```

```txt
lcd(1;7)

Factors of 1 = 1
Factors of 7 = 7

Thus lcd(1;7) = 1 * 7 = 7 (so denominator must be 7)

multiplying fractions in cross:

1 + Â³â„â‚‡ becomes â·â„â‚‡ + Â³â„â‚‡ (makes total sense)

â·â„â‚‡ + Â³â„â‚‡ = â½â·âºÂ³â¾â„â‚‡
         = Â¹â°â„â‚‡
         = 1Â³â„â‚‡

Thus 1 + Â³â„â‚‡ = 1Â³â„â‚‡
```

## Series No. VIII

Resolve:

I) ğŸ ª 4 - Â¹â„â‚‡  
II) ğŸ ª 1Â³â„â‚… - Â²â„â‚ƒ  
III) ğŸ ª 3Â¹â„â‚‚ - 2Â³â„â‚…  
IV) ğŸ ª 1Â³â„â‚‡ - â´â„â‚…  

### Resolution for series no. VIII

```txt
lcd(1;7)

Factors of 1 = 1
Factors of 7 = 7

Thus lcd(1;7) = 1 * 7 = 7 (so denominator must be 7)

multiplying fractions in cross:

4 - Â¹â„â‚‡ becomes Â²â¸â„â‚‡ - Â¹â„â‚‡ (makes total sense)

Â²â¸â„â‚‡ - Â¹â„â‚‡ = â½Â²â¸â»Â¹â¾â„â‚‡
          = Â²â·â„â‚‡
          = 3â¶â„â‚‡

Thus 4 - Â¹â„â‚‡ = 3â¶â„â‚‡
```

```txt
lcd(3;5)

Factors of 3 = 3
Factors of 5 = 5

Thus lcd(3;5) = 3 * 5 = 15 (so denominator must be 15)

1Â³â„â‚… - Â²â„â‚ƒ = â¸â„â‚… - Â²â„â‚ƒ

multiplying fractions in cross:

â¸â„â‚… - Â²â„â‚ƒ becomes Â²â´â„â‚â‚… - Â¹â°â„â‚â‚… (makes total sense)

Â²â´â„â‚â‚… - Â¹â°â„â‚â‚… = â½Â²â´â»Â¹â°â¾â„â‚â‚…
             = Â¹â´â„â‚â‚…

Thus 1Â³â„â‚… - Â²â„â‚ƒ = Â¹â´â„â‚â‚…
```

```txt
lcd(3;5)

Factors of 2 = 2
Factors of 5 = 5

Thus lcd(3;5) = 2 * 5 = 10 (so denominator must be 10)

3Â¹â„â‚‚ - 2Â³â„â‚… = â·â„â‚‚ - Â¹Â³â„â‚…

multiplying fractions in cross:

â·â„â‚‚ - Â¹Â³â„â‚… becomes Â³âµâ„â‚â‚€ - Â²â¶â„â‚â‚€ (makes total sense)

Â³âµâ„â‚â‚€ - Â²â¶â„â‚â‚€ = â½Â³âµâ»Â²â¶â¾â„â‚â‚€
             = â¹â„â‚â‚€

Thus 3Â¹â„â‚‚ - 2Â³â„â‚… = â¹â„â‚â‚€
```

```txt
lcd(5;7)

Factors of 5 = 5
Factors of 7 = 7

Thus lcd(5;7) = 5 * 7 = 35 (so denominator must be 35)

1Â³â„â‚‡ - â´â„â‚… = Â¹â°â„â‚‡ - â´â„â‚…

multiplying fractions in cross:

Â¹â°â„â‚‡ - â´â„â‚… becomes âµâ°â„â‚ƒâ‚… - Â²â¸â„â‚ƒâ‚… (makes total sense)

âµâ°â„â‚ƒâ‚… - Â²â¸â„â‚ƒâ‚… = â½âµâ°â»Â²â¸â¾â„â‚ƒâ‚…
             = Â²Â²â„â‚ƒâ‚…

Thus 1Â³â„â‚‡ - â´â„â‚… = Â²Â²â„â‚ƒâ‚…
```
